code/ecdsap256/Hacl.Impl.SolinasReduction.fsti
@@ -20,4 +20,4 @@ open FStar.Mul
 val solinas_reduction_impl: i: lbuffer uint64 (size 8) -> o: lbuffer uint64 (size 4) -> 
   Stack unit
     (requires fun h -> live h i /\ live h o /\ disjoint i o)
-    (ensures fun h0 _ h1 -> modifies1 o h0 h1 /\ wide_as_nat #P256 h0 i % prime == as_nat P256 h1 o)
+    (ensures fun h0 _ h1 -> modifies1 o h0 h1 /\ wide_as_nat P256 h0 i % prime == as_nat P256 h1 o)
